\documentclass[preview]{standalone}
\usepackage{amsmath}
\usepackage{xcolor}
\usepackage{cancel}
\usepackage{mathtools}

\usepackage[margin=0.5in]{geometry}

\begin{document}

\color{white}

Let $u = k^2 \sin^2 \theta$, and the integrand becomes:
\begin{align*}
  f^{(0)}(u) &=
  \overbrace{(1-u)^{-\frac{1}{2}}}^{\mathclap{\text{binomial series $(1+x)^k =
  \sum_{n=0}^{\infty} \binom{k}{n} x^n$}}} &&\rightarrow f^{(0)}(0) =
  \frac{1}{\cancel{2^0}} \\
  f^{(1)}(u) &= -\frac{1}{2} (1-u)^{-\frac{3}{2}} (-1) &&\rightarrow
  f^{(1)}(0) = \frac{1}{2^1} \\
  f^{(2)}(u) &= -\frac{1\cdot3}{2^2} (1-u)^{-\frac{5}{2}} (-1)
  &&\rightarrow f^{(2)}(0) = \frac{1\cdot3}{2^2} \\
  f^{(3)}(u) &=
  -\frac{\color{cyan}\overbrace{1\cdot3\cdot5}^{\mathclap{\text{odd-only
  factorial}}}}{\color{pink}2^3} (1-u)^{\color{yellow} -\frac{7}{2}} (-1)
  &&\rightarrow f^{(3)}(0) =
  \frac{1\cdot3\cdot5}{2^3} \\
  f^{(n)}(u) &= \frac{{\color{cyan}(2n-1)!!}}{{\color{pink}2^n}}
  (1-u)^{\color{yellow} -\frac{2n+1}{2}}
  &&\rightarrow f^{(n)}(0) = \frac{{(2n-1)!!}}{{2^n}}
\end{align*}
Plugging in to the Maclaurin series formula $f(x) =
\sum_{n=0}^{\infty} \frac{f^{(n)}(0)}{n!} x^n$, we get:
\[
  \frac{1}{\sqrt{1 - u}} = \sum_{n=0}^{\infty} \frac{
  (2n-1)!!}{\color{orange}\underbrace{2^n n!}_{\mathclap{2 \cdot 1 +
  2 \cdot 2 + 2 \cdot 3 + \cdots = 2 \cdot 4 \cdot 6 \cdots}}} u^n =
  \sum_{n=0}^{\infty} \frac{(2n-1)!!}{\color{orange} (2n)!!}
  {\left(k\sin\theta\right)}^{2n}
\]
For $n = 0$, $(2(0) - 1)!! = (-1)!! = 1$ by
convention.

\end{document}